theories/TM/PCTM.v
@@ -21,6 +21,7 @@ Set Implicit Arguments.
 
 (** * Halting problem for (micro-programmed) Turing machines with a PC counter *)
 
+(* Four instructions: MV d | WR b | JZ i | JMP i *)
 Inductive pctm_instr : Set :=
   | pctm_mv  : direction -> pctm_instr
   | pctm_wr  : bool -> pctm_instr
@@ -34,32 +35,44 @@ Module PCTMNotations.
   Notation JZ  := pctm_jz.
   Notation JMP := pctm_jmp.
 
-  Definition rd (t : tape) : bool := let '(_,b,_) := t in b.
+  Definition rd (t : tape) : bool   := let '(_,b,_) := t in b.
   Definition wr (t : tape) b : tape := let '(l,_,r) := t in (l,b,r).
 
 End PCTMNotations.
 
 Import PCTMNotations SBTMNotations.
 
-(* ** Semantics for PC based TM *)
+(* ** Small-step semantics for PC based TM *)
 
-Section PC_based_Single_Tape_Turing_Machine.
+(* state is a value for the PC value and a tape *) 
+Definition pctm_state := (nat * tape)%type.
 
-  Definition pctm_state := (nat*tape)%type.
+(**    ρ // (i,t₁) -1> (j,t₂) 
+    means instruction ρ at PC i transforms 
+    the state (i,t₁) into the state (j,t₂) *)
 
-  Inductive pctm_sss : pctm_instr -> pctm_state -> pctm_state -> Prop :=
-    | pctm_sss_mv d i t :   MV d // (i,t) -1> (1+i,mv d t)       (* From the SBTM.v *)
-    | pctm_sss_wr b i t :   WR b // (i,t) -1> (1+i,wr t b)
-    | pctm_sss_jz i j t :   JZ j // (i,t) -1> (if rd t then 1+i else j,t)
-    | pctm_sss_jmp i j t : JMP j // (i,t) -1> (j,t)
-  where "i // s -1> t" := (pctm_sss i s t).
+Inductive pctm_sss : pctm_instr -> pctm_state -> pctm_state -> Prop :=
+  | pctm_sss_mv d i t :   MV d // (i,t) -1> (1+i,mv d t)       (* mv is from the TM/SBTM.v *)
+  | pctm_sss_wr b i t :   WR b // (i,t) -1> (1+i,wr t b)
+  | pctm_sss_jz i j t :   JZ j // (i,t) -1> (if rd t then 1+i else j,t)
+  | pctm_sss_jmp i j t : JMP j // (i,t) -1> (j,t)
+where "ρ // s -1> t" := (pctm_sss ρ s t).
 
-End PC_based_Single_Tape_Turing_Machine.
+(** when P = (i,l) with (i = start PC value for instructions in l) 
+                  and  (l = list of instructions)
+   P // s ↓ means repeating steps as above in P, starting from s,
+   eventually leads to a PC value outside of P
 
-(* The Halting problem for PCTM *)
-  
-Definition PCTM_PROBLEM := (list pctm_instr * tape)%type.
+   Notice that this is equivalent to termination because the PCTM
+   small steps semantics is total, ie if there is an instruction at
+   the current PC, then a computation step can occur: no instruction
+   is blocking *)
 
 #[local] Notation "P // s ↓" := (sss_terminates pctm_sss P s).
 
-Definition PCTM_HALT (Q : PCTM_PROBLEM) := let (P,t) := Q in (1,P) // (1,t) ↓.
+(* ** The Halting problem for PCTM *)
+  
+Definition PCTM_PROBLEM := (list pctm_instr * tape)%type.
+
+Definition PCTM_HALT (Q : PCTM_PROBLEM) :=
+  let (P,t) := Q in (1,P) // (1,t) ↓.
